Anon3Assignment.lean
@@ -1,1 +1,13 @@
 import Anon3Assignment.Grader
+import Anon3Assignment.Student
+
+#eval Anon3.runImplementation Anon3.Student.implementation 3 1 [
+  .add 3,
+  .add 1,
+  .calc,
+  .add 10,
+  .calc,
+  .add 5,
+  .add 5,
+  .add 5,
+  .calc]
